Algorithm.lean
@@ -1,7 +1,6 @@
 import Algorithm.Algebra.BigOperators.DFinsupp'
 import Algorithm.Data.Classes.AssocArray
 import Algorithm.Data.Classes.Bag
-import Algorithm.Data.Classes.DynamicArrayLike
 import Algorithm.Data.Classes.IndexedMinHeap
 import Algorithm.Data.Classes.MinHeap
 import Algorithm.Data.Classes.MultiBag
